theories/Int63/vst/proof/proof.v
@@ -6,441 +6,455 @@ From VST Require Import floyd.proofauto.
 
 
 Module Facts.
-    Lemma encode_Z_bitwise (x: Z):
-        Int64.repr (encode_Z x) = Int64.or (Int64.shl (Int64.repr x) (Int64.repr 1)) (Int64.repr 1).
-    Proof.
-        rewrite Int64.shifted_or_is_add.
-        2: { constructor ; try lia ; try constructor. }
-        2: { constructor. }
-        assert (E: two_p 1 = Int64.unsigned (Int64.repr 2)). { reflexivity. } rewrite E ; clear E.
+  Lemma encode_Z_bounds (x: Z) (Hx: Int64.min_signed <= encode_Z x <= Int64.max_signed):
+    Int64.min_signed <= x <= Int64.max_signed.
+  Proof.
+    change Int64.min_signed with (- 2^63) in *.
+    change Int64.max_signed with (2^63 - 1) in *.
+    apply encode_Z__bounds ; lia.
+  Qed.
 
-        unfold encode_Z.
-        repeat rewrite <- add64_repr.
-        repeat rewrite <- mul64_repr.
-        assert (E: forall z, Int64.repr (Int64.unsigned (Int64.repr z)) = Int64.repr z).
-        {
-            intro z.
-            symmetry.
-            apply Int64.eqm_samerepr.
-            apply Int64.eqm_unsigned_repr.
-        } repeat rewrite E ; clear E.
+
+  Lemma encode_Z_bitwise (x: Z):
+    Int64.repr (encode_Z x) = Int64.or (Int64.shl (Int64.repr x) (Int64.repr 1)) (Int64.repr 1).
+  Proof.
+    rewrite Int64.shifted_or_is_add.
+    2: { constructor ; try lia ; try constructor. }
+    2: { constructor. }
+    assert (E: two_p 1 = Int64.unsigned (Int64.repr 2)). { reflexivity. } rewrite E ; clear E.
+
+    unfold encode_Z.
+    repeat rewrite <- add64_repr.
+    repeat rewrite <- mul64_repr.
+    assert (E: forall z, Int64.repr (Int64.unsigned (Int64.repr z)) = Int64.repr z).
+    {
+      intro z.
+      symmetry.
+      apply Int64.eqm_samerepr.
+      apply Int64.eqm_unsigned_repr.
+    } repeat rewrite E ; clear E.
+    reflexivity.
+  Qed.
+
+  Lemma decode_Z_sign_bit (x: Z) (Hx: Int64.min_signed <= encode_Z x <= Int64.max_signed):
+    Int64.testbit (Int64.repr x) (Int64.zwordsize - 1) =
+    Int64.testbit (Int64.repr x) (Int64.zwordsize - 1 - 1).
+  Proof.
+    repeat rewrite Int64.testbit_repr.
+    2: { cbv. constructor ; congruence. }
+    2: { cbv. constructor ; congruence. }
+    destruct x as [ | x' | x' ] ; try reflexivity.
+    {
+      assert (H': Z.log2 (Z.pos x') < Int64.zwordsize - 1 - 1).
+      2: { repeat rewrite Z.bits_above_log2 ; try lia. }
+      destruct Hx as [ Hx_l Hx_h ].
+      clear Hx_l.
+      apply Z.log2_le_mono in Hx_h.
+
+      assert (E: Int64.zwordsize - 1 - 1 = 62). { reflexivity. } rewrite E in * ; clear E.
+      assert (E: Z.log2 Int64.max_signed = 62). { reflexivity. } rewrite E in * ; clear E.
+
+      assert (E: Z.log2 (Z.pos x') = Z.log2 (encode_Z (Z.pos x')) - 1).
+      2: { rewrite E. lia. }
+
+      rewrite encode_Z__bitwise.
+      simpl Z.shiftl.
+      simpl Z.lor.
+
+      transitivity (Z.pos (Pos.size x') - 1).
+      2: { reflexivity. }
+      clear Hx_h.
+      destruct x' ; try reflexivity.
+      all: simpl Pos.size ; simpl Z.log2 ; lia.
+    }
+    {
+      assert (Hx_l: Int64.min_signed < encode_Z (Z.neg x')).
+      {
+        change Int64.min_signed with (- 2^63) in *.
+        apply encode_Z__tight_lower_bound ; try lia.
+      }
+      unfold encode_Z in Hx_l.
+      assert (H': Z.pos x' * 2 - 1 <= - Int64.min_signed - 1) by lia.
+      clear Hx_l. rename H' into Hx_l.
+
+      apply Z.log2_le_mono in Hx_l.
+
+      change (Int64.zwordsize - 1 - 1) with 62 in *.
+      change (Int64.zwordsize - 1) with 63 in *.
+      change (Z.log2 (- Int64.min_signed - 1)) with 62 in *.
+
+      assert (H'': Z.log2 (Z.pos x') <= Z.log2 (Z.pos x' * 2 - 1)).
+      {
+        apply Z.log2_le_mono.
+        lia.  
+      }
+
+      transitivity true.
+      { apply Z.bits_iff_neg ; try simpl Z.abs ; try lia. }
+      symmetry.
+
+      assert (Hx': Z.pos x' <= two_power_nat 62).
+      {
+        change Int64.min_signed with (- ((two_power_nat 62) * 2)) in *.
+        unfold encode_Z in Hx.
+        lia.
+      }
+      clear Hx. rename Hx' into Hx.
+      assert (Hx': Z.pos x' < two_power_nat 62 \/ Z.pos x' = two_power_nat 62). { lia. }
+      clear Hx. rename Hx' into Hx.
+
+      destruct Hx as [ Hx | Hx ].
+      {
+        apply Z.bits_iff_neg ; try lia.
+        simpl Z.abs.
+        assert (Hx': Z.pos x' <= two_power_nat 62 - 1). { lia. } clear Hx. rename Hx' into Hx.
+        apply Z.log2_le_mono in Hx.
+        change (Z.log2 (two_power_nat 62 - 1)) with 61 in *.
+        lia.
+      }
+      {
+        inversion Hx.
         reflexivity.
-    Qed.
+      }
+    }
+  Qed.
 
-    Lemma decode_Z_sign_bit (x: Z) (Hx: Int64.min_signed <= encode_Z x <= Int64.max_signed):
-        Int64.testbit (Int64.repr x) (Int64.zwordsize - 1) =
-        Int64.testbit (Int64.repr x) (Int64.zwordsize - 1 - 1).
-    Proof.
-        repeat rewrite Int64.testbit_repr.
-        2: { cbv. constructor ; congruence. }
-        2: { cbv. constructor ; congruence. }
-        destruct x as [ | x' | x' ] ; try reflexivity.
-        {
-            assert (H': Z.log2 (Z.pos x') < Int64.zwordsize - 1 - 1).
-            2: { repeat rewrite Z.bits_above_log2 ; try lia. }
-            destruct Hx as [ Hx_l Hx_h ].
-            clear Hx_l.
-            apply Z.log2_le_mono in Hx_h.
+  Lemma decode_Z_sign_ext (x: Z) (Hx: Int64.min_signed <= encode_Z x <= Int64.max_signed):
+    Int64.repr x =
+    Int64.sign_ext (Int64.zwordsize - Int64.unsigned (Int64.repr 1)) (Int64.repr x).
+  Proof.
+    apply Int64.same_bits_eq. intros i Hi.
+    assert (E: Int64.unsigned (Int64.repr 1) = 1). { reflexivity. } rewrite E ; clear E.
+    rewrite Int64.bits_sign_ext ; try assumption.
+    destruct (zlt i (Int64.zwordsize - 1)) as [ _ | Hi' ] ; try reflexivity.
+    assert (Hi'': forall z, i >= z -> i > z \/ i = z). { lia. } apply Hi'' in Hi' ; clear Hi''.
+    destruct Hi' as [ Hi' | Hi' ] ; try lia.
+    subst.
+    apply decode_Z_sign_bit.
+    assumption.
+  Qed.
 
-            assert (E: Int64.zwordsize - 1 - 1 = 62). { reflexivity. } rewrite E in * ; clear E.
-            assert (E: Z.log2 Int64.max_signed = 62). { reflexivity. } rewrite E in * ; clear E.
-
-            assert (E: Z.log2 (Z.pos x') = Z.log2 (encode_Z (Z.pos x')) - 1).
-            2: { rewrite E. lia. }
-
-            rewrite encode_Z.bitwise.
-            simpl Z.shiftl.
-            simpl Z.lor.
-
-            transitivity (Z.pos (Pos.size x') - 1).
-            2: { reflexivity. }
-            clear Hx_h.
-            destruct x' ; try reflexivity.
-            all: simpl Pos.size ; simpl Z.log2 ; lia.
-        }
-        {
-            apply encode_Z.tight_bound in Hx.
-            unfold encode_Z in Hx.
-            assert (H': Z.pos x' * 2 - 1 < - Int64.min_signed). { lia. }
-            rename H' into Hx_l.
-
-            assert (H': Z.pos x' * 2 - 1 <= - Int64.min_signed - 1). { lia. }
-            clear Hx_l. rename H' into Hx_l.
-
-            apply Z.log2_le_mono in Hx_l.
-
-            assert (E: Int64.zwordsize - 1 - 1 = 62). { reflexivity. } rewrite E in * ; clear E.
-            assert (E: Int64.zwordsize - 1 = 63). { reflexivity. } rewrite E in * ; clear E.
-            assert (E: Z.log2 (- Int64.min_signed - 1) = 62). { reflexivity. } rewrite E in * ; clear E.
-
-            assert (H'': Z.log2 (Z.pos x') <= Z.log2 (Z.pos x' * 2 - 1)).
-            {
-                apply Z.log2_le_mono.
-                lia.    
-            }
-
-            transitivity true.
-            { apply Z.bits_iff_neg ; try simpl Z.abs ; try lia. }
-            symmetry.
-
-            assert (Hx': Z.pos x' <= two_power_nat 62).
-            {
-                assert (E: Int64.min_signed = - ((two_power_nat 62) * 2)). { reflexivity. } rewrite E in * ; clear E.
-                lia.
-            }
-            clear Hx. rename Hx' into Hx.
-            assert (Hx': Z.pos x' < two_power_nat 62 \/ Z.pos x' = two_power_nat 62). { lia. }
-            clear Hx. rename Hx' into Hx.
-
-            destruct Hx as [ Hx | Hx ].
-            {
-                apply Z.bits_iff_neg ; try lia.
-                simpl Z.abs.
-                assert (Hx': Z.pos x' <= two_power_nat 62 - 1). { lia. } clear Hx. rename Hx' into Hx.
-                apply Z.log2_le_mono in Hx.
-                assert (E: Z.log2 (two_power_nat 62 - 1) = 61). { reflexivity. } rewrite E in * ; clear E.
-                lia.
-            }
-            {
-                inversion Hx.
-                reflexivity.
-            }
-        }
-    Qed.
-
-    Lemma decode_Z_sign_ext (x: Z) (Hx: Int64.min_signed <= encode_Z x <= Int64.max_signed):
-        Int64.repr x =
-        Int64.sign_ext (Int64.zwordsize - Int64.unsigned (Int64.repr 1)) (Int64.repr x).
-    Proof.
-        apply Int64.same_bits_eq. intros i Hi.
-        assert (E: Int64.unsigned (Int64.repr 1) = 1). { reflexivity. } rewrite E ; clear E.
-        rewrite Int64.bits_sign_ext ; try assumption.
-        destruct (zlt i (Int64.zwordsize - 1)) as [ _ | Hi' ] ; try reflexivity.
-        assert (Hi'': forall z, i >= z -> i > z \/ i = z). { lia. } apply Hi'' in Hi' ; clear Hi''.
-        destruct Hi' as [ Hi' | Hi' ] ; try lia.
-        subst.
-        apply decode_Z_sign_bit.
-        assumption.
-    Qed.
-
-    Lemma decode_Z_bitwise (x: Z) (Hx: Int64.min_signed <= encode_Z x <= Int64.max_signed):
-        Int64.repr x = Int64.shr (Int64.repr (encode_Z x)) (Int64.repr 1).
-    Proof.
-        rewrite encode_Z_bitwise.
-        rewrite <- Int64.or_shr.
-        assert (E: Int64.shr (Int64.repr 1) (Int64.repr 1) = Int64.zero). { reflexivity. } rewrite E ; clear E.
-        rewrite Int64.or_zero.
-        rewrite Int64.shr_shl.
-        2: { reflexivity. }
-        2: { reflexivity. }
-        assert (E: Int64.ltu (Int64.repr 1) (Int64.repr 1) = false). { reflexivity. } rewrite E ; clear E.
-        assert (E: Int64.sub (Int64.repr 1) (Int64.repr 1) = Int64.zero). { reflexivity. } rewrite E ; clear E.
-        rewrite Int64.shr_zero.
-        apply decode_Z_sign_ext.
-        assumption.
-    Qed.
+  Lemma decode_Z_bitwise (x: Z) (Hx: Int64.min_signed <= encode_Z x <= Int64.max_signed):
+    Int64.repr x = Int64.shr (Int64.repr (encode_Z x)) (Int64.repr 1).
+  Proof.
+    rewrite encode_Z_bitwise.
+    rewrite <- Int64.or_shr.
+    assert (E: Int64.shr (Int64.repr 1) (Int64.repr 1) = Int64.zero). { reflexivity. } rewrite E ; clear E.
+    rewrite Int64.or_zero.
+    rewrite Int64.shr_shl.
+    2: { reflexivity. }
+    2: { reflexivity. }
+    assert (E: Int64.ltu (Int64.repr 1) (Int64.repr 1) = false). { reflexivity. } rewrite E ; clear E.
+    assert (E: Int64.sub (Int64.repr 1) (Int64.repr 1) = Int64.zero). { reflexivity. } rewrite E ; clear E.
+    rewrite Int64.shr_zero.
+    apply decode_Z_sign_ext.
+    assumption.
+  Qed.
 End Facts.
 
 
 Lemma encode_int63_body: semax_body Vprog ASI f_encode_int63 encode_int63_spec.
-    leaf_function.
-    start_function.
-    repeat forward ; entailer!.
-    rewrite Facts.encode_Z_bitwise ; trivial.
+  leaf_function.
+  start_function.
+  repeat forward ; entailer!.
+  rewrite Facts.encode_Z_bitwise ; trivial.
 Qed.
 
 Lemma decode_int63_body: semax_body Vprog ASI f_decode_int63 decode_int63_spec.
-    leaf_function.
-    start_function.
-    repeat forward ; entailer!.
-    symmetry.
-    rewrite Facts.decode_Z_bitwise ; trivial.
+  leaf_function.
+  start_function.
+  repeat forward ; entailer!.
+  symmetry.
+  rewrite Facts.decode_Z_bitwise ; trivial.
 Qed.
 
 Lemma int63_zero_body: semax_body Vprog ASI f_int63_zero int63_zero_spec.
 Proof.
-    start_function.
-    repeat step.
+  start_function.
+  repeat step.
 Qed.
 
 Lemma int63_one_body: semax_body Vprog ASI f_int63_one int63_one_spec.
 Proof.
-    start_function.
-    repeat step.
+  start_function.
+  repeat step.
 Qed.
 
 Lemma int63_neg_body: semax_body Vprog ASI f_int63_neg int63_neg_spec.
 Proof.
-    start_function.
-    repeat step ; entailer!.
-    {
-        apply encode_Z.tight_bound in H0.
-        unfold encode_Z in *.
-        lia.
-    }
-    simpl.
-    repeat f_equal.
-    unfold encode_Z.
+  start_function.
+  repeat step ; entailer!.
+  {
+    unfold encode_Z in *.
     lia.
+  }
+  simpl.
+  repeat f_equal.
+  unfold encode_Z.
+  lia.
 Qed.
 
 Lemma int63_abs_body: semax_body Vprog ASI f_int63_abs int63_abs_spec.
 Proof.
-    start_function.
-    forward_if (PROP () LOCAL (temp _t'1 (Vlong (Int64.repr (encode_Z (Z.abs x))))) SEP ()).
-    {
-        repeat step.
-        entailer!.
-        repeat f_equal.
-        intros.
-        rewrite Int64.signed_repr in H1 ; try lia.
-        assert (E: Int64.signed (Int64.repr 0) = 0). { reflexivity. } rewrite E in * ; clear E.
-        unfold encode_Z in *.
-        rewrite <- Z.abs_opp.
-        rewrite Z.abs_eq ; try lia.
-    }
-    {
-        repeat step.
-        entailer!.
-        repeat f_equal.
-        rewrite Int64.signed_repr in H1 ; try lia.
-        assert (E: Int64.signed (Int64.repr 0) = 0). { reflexivity. } rewrite E in * ; clear E.
-        unfold encode_Z in *.
-        apply Z.abs_eq.
-        lia.
-    }
+  start_function.
+  forward_if (PROP () LOCAL (temp _t'1 (Vlong (Int64.repr (encode_Z (Z.abs x))))) SEP ()).
+  {
     repeat step.
+    entailer!.
+    repeat f_equal.
+    intros.
+    rewrite Int64.signed_repr in H1 ; try lia.
+    assert (E: Int64.signed (Int64.repr 0) = 0). { reflexivity. } rewrite E in * ; clear E.
+    unfold encode_Z in *.
+    rewrite <- Z.abs_opp.
+    rewrite Z.abs_eq ; try lia.
+  }
+  {
+    repeat step.
+    entailer!.
+    repeat f_equal.
+    rewrite Int64.signed_repr in H1 ; try lia.
+    assert (E: Int64.signed (Int64.repr 0) = 0). { reflexivity. } rewrite E in * ; clear E.
+    unfold encode_Z in *.
+    apply Z.abs_eq.
+    lia.
+  }
+  repeat step.
 Qed.
 
 Lemma int63_add_body: semax_body Vprog ASI f_int63_add int63_add_spec.
 Proof.
-    leaf_function.
-    start_function.
-    repeat step ; try entailer!.
-    {
-        unfold encode_Z in *.
-        repeat rewrite Int64.signed_repr ; try lia.
-    }
-    {
-        repeat f_equal.
-        unfold encode_Z.
-        lia.
-    }
+  leaf_function.
+  start_function.
+  repeat step ; try entailer!.
+  {
+    unfold encode_Z in *.
+    repeat rewrite Int64.signed_repr ; try lia.
+  }
+  {
+    repeat f_equal.
+    unfold encode_Z.
+    lia.
+  }
 Qed.
 
 Lemma int63_sub_body: semax_body Vprog ASI f_int63_sub int63_sub_spec.
 Proof.
-    leaf_function.
-    start_function.
-    assert (H': Int64.min_signed <= encode_Z (x - y) - 1 <= Int64.max_signed).
+  leaf_function.
+  start_function.
+  assert (H': Int64.min_signed <= encode_Z (x - y) - 1 <= Int64.max_signed).
+  {
+    assert (H_tight: Int64.min_signed < encode_Z (x - y)).
     {
-        apply encode_Z.tight_bound in H1.
-        lia.
+      change Int64.min_signed with (-2^63) in *.
+      apply encode_Z__tight_lower_bound ; lia.
     }
-    repeat step ; try entailer!.
-    {
-        unfold encode_Z in *.
-        repeat rewrite Int64.signed_repr ; try lia.
-    }
-    {
-        repeat f_equal.
-        unfold encode_Z.
-        lia.
-    }
+    lia.
+  }
+  repeat step ; try entailer!.
+  {
+    unfold encode_Z in *.
+    repeat rewrite Int64.signed_repr ; try lia.
+  }
+  {
+    repeat f_equal.
+    unfold encode_Z.
+    lia.
+  }
 Qed.
 
 Lemma int63_mul_body: semax_body Vprog ASI f_int63_mul int63_mul_spec.
 Proof.
-    start_function.
-    repeat step ; try entailer!.
-    repeat rewrite Int64.signed_repr ; apply encode_Z.bound ; assumption.
+  start_function.
+  repeat step ; try entailer!.
+  repeat rewrite Int64.signed_repr ; apply Facts.encode_Z_bounds ; lia.
 Qed.
 
 Lemma int63_div_body: semax_body Vprog ASI f_int63_div int63_div_spec.
 Proof.
-    start_function.
-    repeat step ; try entailer!.
+  start_function.
+  repeat step ; try entailer!.
+  {
+    constructor.
     {
-        constructor.
-        {
-            intro F.
-            apply H1. clear H1.
-            transitivity (Int64.signed (Int64.repr y)).
-            {
-                rewrite Int64.signed_repr ; try apply encode_Z.bound ; trivial.
-            }
-            {
-                rewrite F ; trivial.
-            }
-        }
-        {
-            intro F.
-            assert (E: Int64.signed (Int64.repr x) = Int64.signed (Int64.repr Int64.min_signed)).
-            { destruct F. congruence. }
-            clear F.
-
-            rewrite Int64.signed_repr in E ; try apply encode_Z.bound ; try lia.
-            rewrite Int64.signed_repr in E ; try lia.
-
-            destruct H as [ H H' ]. clear H'.
-            apply H. subst. reflexivity.
-        }
+      intro F.
+      apply H1. clear H1.
+      transitivity (Int64.signed (Int64.repr y)).
+      {
+        rewrite Int64.signed_repr ; try apply Facts.encode_Z_bounds ; lia.
+      }
+      {
+        rewrite F ; trivial.
+      }
     }
     {
-        repeat f_equal ; try rewrite Int64.signed_repr ; try apply encode_Z.bound ; trivial.
+      intro F.
+      assert (E: Int64.signed (Int64.repr x) = Int64.signed (Int64.repr Int64.min_signed)).
+      { destruct F. congruence. }
+      clear F.
+
+      rewrite Int64.signed_repr in E ; try apply Facts.encode_Z_bounds ; try lia.
+      rewrite Int64.signed_repr in E ; try lia.
+
+      destruct H as [ H H' ]. clear H'.
+      apply H. subst. reflexivity.
     }
+  }
+  {
+    repeat f_equal ; try rewrite Int64.signed_repr ; try apply Facts.encode_Z_bounds ; lia.
+  }
 Qed.
 
 Lemma int63_rem_body: semax_body Vprog ASI f_int63_rem int63_rem_spec.
 Proof.
-    start_function.
-    repeat step ; try entailer!.
+  start_function.
+  repeat step ; try entailer!.
+  {
+    constructor.
     {
-        constructor.
-        {
-            intro F.
-            apply H1.
-            transitivity (Int64.signed (Int64.repr y)).
-            {
-                rewrite Int64.signed_repr ; try apply encode_Z.bound ; trivial.
-            }
-            {
-                rewrite F ; trivial.
-            }
-        }
-        {
-            intro F.
-            assert (E: Int64.signed (Int64.repr x) = Int64.signed (Int64.repr Int64.min_signed)).
-            { destruct F. congruence. }
-            clear F.
-
-            rewrite Int64.signed_repr in E ; try apply encode_Z.bound ; try lia.
-            rewrite Int64.signed_repr in E ; try lia.
-
-            destruct H as [ H H' ]. clear H'.
-            apply H. subst. reflexivity.
-        }
+      intro F.
+      apply H1.
+      transitivity (Int64.signed (Int64.repr y)).
+      {
+        rewrite Int64.signed_repr ; try apply Facts.encode_Z_bounds ; trivial.
+      }
+      {
+        rewrite F ; trivial.
+      }
     }
     {
-        repeat f_equal ; try rewrite Int64.signed_repr ; try apply encode_Z.bound ; trivial.
+      intro F.
+      assert (E: Int64.signed (Int64.repr x) = Int64.signed (Int64.repr Int64.min_signed)).
+      { destruct F. congruence. }
+      clear F.
+
+      rewrite Int64.signed_repr in E ; try apply Facts.encode_Z_bounds ; try lia.
+      rewrite Int64.signed_repr in E ; try lia.
+
+      destruct H as [ H H' ]. clear H'.
+      apply H. subst. reflexivity.
     }
+  }
+  {
+    repeat f_equal ; try rewrite Int64.signed_repr ; try apply Facts.encode_Z_bounds ; trivial.
+  }
 Qed.
 
 Lemma int63_shiftl_body: semax_body Vprog ASI f_int63_shiftl int63_shiftl_spec.
 Proof.
-    start_function.
-    repeat step ; try entailer!.
-    {
-        unfold Int64.iwordsize.
-        rewrite Int64.unsigned_repr ; try lia.
-        constructor ; cbv ; congruence.
-    }
-    {
-        apply encode_Z.bound in H.
-        generalize Int64.max_signed_unsigned. intro.
-        generalize (Int64.unsigned_range_2 (Int64.repr y)). intro.
-        assert (H': Int64.zwordsize <= Int64.max_signed). { intro F. inversion F. }
-        repeat f_equal ; rewrite Int64.unsigned_repr in * ; try lia.
-    }
+  start_function.
+  repeat step ; try entailer!.
+  {
+    unfold Int64.iwordsize.
+    rewrite Int64.unsigned_repr ; try lia.
+    constructor ; cbv ; congruence.
+  }
+  {
+    apply Facts.encode_Z_bounds in H.
+    generalize Int64.max_signed_unsigned. intro.
+    generalize (Int64.unsigned_range_2 (Int64.repr y)). intro.
+    assert (H': Int64.zwordsize <= Int64.max_signed). { intro F. inversion F. }
+    repeat f_equal ; rewrite Int64.unsigned_repr in * ; try lia.
+  }
 Qed.
 
 Lemma int63_shiftr_body: semax_body Vprog ASI f_int63_shiftr int63_shiftr_spec.
 Proof.
-    start_function.
-    repeat step ; try entailer!.
-    {
-        unfold Int64.iwordsize.
-        rewrite Int64.unsigned_repr ; try lia.
-        constructor ; cbv ; congruence.
-    }
-    {
-        repeat f_equal ; rewrite Int64.signed_repr ; try apply encode_Z.bound ; trivial.
-    }
+  start_function.
+  repeat step ; try entailer!.
+  {
+    unfold Int64.iwordsize.
+    rewrite Int64.unsigned_repr ; try lia.
+    constructor ; cbv ; congruence.
+  }
+  {
+    repeat f_equal ; rewrite Int64.signed_repr ; try apply Facts.encode_Z_bounds ; trivial.
+  }
 Qed.
 
 Lemma int63_or_body: semax_body Vprog ASI f_int63_or int63_or_spec.
 Proof.
-    leaf_function.
-    start_function.
-    repeat step ; try entailer!.
-    repeat f_equal.
-    repeat rewrite encode_Z.bitwise.
+  leaf_function.
+  start_function.
+  repeat step ; try entailer!.
+  repeat f_equal.
+  repeat rewrite encode_Z__bitwise.
 
-    rewrite <- Z.lor_assoc.
-    assert (E: Z.lor (Z.shiftl x 1) (Z.lor 1 (Z.shiftl y 1)) = Z.lor 1 (Z.lor (Z.shiftl x 1) (Z.shiftl y 1))).
-    {
-        rewrite Z.lor_assoc.
-        rewrite Z.lor_assoc.
-        assert (E: Z.lor (Z.shiftl x 1) 1 = Z.lor 1 (Z.shiftl x 1)). { apply Z.lor_comm. } rewrite E ; clear E.
-        reflexivity.
-    } rewrite E ; clear E.
+  rewrite <- Z.lor_assoc.
+  assert (E: Z.lor (Z.shiftl x 1) (Z.lor 1 (Z.shiftl y 1)) = Z.lor 1 (Z.lor (Z.shiftl x 1) (Z.shiftl y 1))).
+  {
     rewrite Z.lor_assoc.
-    rewrite Z.shiftl_lor.
+    rewrite Z.lor_assoc.
+    assert (E: Z.lor (Z.shiftl x 1) 1 = Z.lor 1 (Z.shiftl x 1)). { apply Z.lor_comm. } rewrite E ; clear E.
     reflexivity.
+  } rewrite E ; clear E.
+  rewrite Z.lor_assoc.
+  rewrite Z.shiftl_lor.
+  reflexivity.
 Qed.
 
 Lemma int63_and_body: semax_body Vprog ASI f_int63_and int63_and_spec.
 Proof.
-    leaf_function.
-    start_function.
-    repeat step ; try entailer!.
-    repeat f_equal.
-    repeat rewrite encode_Z.bitwise.
+  leaf_function.
+  start_function.
+  repeat step ; try entailer!.
+  repeat f_equal.
+  repeat rewrite encode_Z__bitwise.
 
-    repeat rewrite Z.land_lor_distr_l.
-    repeat rewrite Z.land_lor_distr_r.
-    assert (E: Z.land 1 1 = 1). { reflexivity. } repeat rewrite E ; clear E.
-    assert (E: forall z, Z.land z 1 = Z.land 1 z). { intros ; apply Z.land_comm. } repeat rewrite E ; clear E.
-    assert (E: forall z, Z.land 1 (Z.shiftl z 1) = 0).
-    {
-        destruct z ; try reflexivity.
-        destruct p ; try reflexivity.
-    } repeat rewrite E ; clear E.
-    f_equal.
-    rewrite Z.lor_0_l.
-    rewrite Z.shiftl_land.
-    reflexivity.
+  repeat rewrite Z.land_lor_distr_l.
+  repeat rewrite Z.land_lor_distr_r.
+  assert (E: Z.land 1 1 = 1). { reflexivity. } repeat rewrite E ; clear E.
+  assert (E: forall z, Z.land z 1 = Z.land 1 z). { intros ; apply Z.land_comm. } repeat rewrite E ; clear E.
+  assert (E: forall z, Z.land 1 (Z.shiftl z 1) = 0).
+  {
+    destruct z ; try reflexivity.
+    destruct p ; try reflexivity.
+  } repeat rewrite E ; clear E.
+  f_equal.
+  rewrite Z.lor_0_l.
+  rewrite Z.shiftl_land.
+  reflexivity.
 Qed.
 
 Lemma int63_xor_body: semax_body Vprog ASI f_int63_xor int63_xor_spec.
 Proof.
-    leaf_function.
-    start_function.
-    repeat step ; try entailer!.
-    repeat rewrite encode_Z.bitwise.
-    repeat rewrite <- or64_repr.
-    repeat f_equal.
+  leaf_function.
+  start_function.
+  repeat step ; try entailer!.
+  repeat rewrite encode_Z__bitwise.
+  repeat rewrite <- or64_repr.
+  repeat f_equal.
 
-    apply Int64.same_bits_eq.
-    intros i Hi.
-    rewrite Z.shiftl_lxor.
-    repeat rewrite Int64.bits_xor ; try assumption.
-    repeat rewrite Int64.bits_or ; try assumption.
-    repeat rewrite Int64.testbit_repr ; try assumption.
-    repeat rewrite Z.lxor_spec.
-    repeat rewrite Z.shiftl_spec ; try lia.
-    destruct i as [ | i' | i' ] ; trivial.
+  apply Int64.same_bits_eq.
+  intros i Hi.
+  rewrite Z.shiftl_lxor.
+  repeat rewrite Int64.bits_xor ; try assumption.
+  repeat rewrite Int64.bits_or ; try assumption.
+  repeat rewrite Int64.testbit_repr ; try assumption.
+  repeat rewrite Z.lxor_spec.
+  repeat rewrite Z.shiftl_spec ; try lia.
+  destruct i as [ | i' | i' ] ; trivial.
 Qed.
 
 Lemma int63_not_body: semax_body Vprog ASI f_int63_not int63_not_spec.
 Proof.
-    leaf_function.
-    start_function.
-    repeat step ; try entailer!.
-    repeat rewrite encode_Z.bitwise.
-    unfold Int64.not.
-    repeat rewrite <- or64_repr.
-    repeat f_equal.
+  leaf_function.
+  start_function.
+  repeat step ; try entailer!.
+  repeat rewrite encode_Z__bitwise.
+  unfold Int64.not.
+  repeat rewrite <- or64_repr.
+  repeat f_equal.
 
-    apply Int64.same_bits_eq.
-    intros i Hi.
-    repeat rewrite Int64.bits_xor ; try assumption.
-    repeat rewrite Int64.bits_or ; try assumption.
-    unfold Int64.mone.
-    repeat rewrite Int64.testbit_repr ; try assumption.
-    repeat rewrite Z.shiftl_spec ; try lia.
-    destruct i as [ | i' | i' ] ; try reflexivity.
-    repeat rewrite Z.lnot_spec ; try lia.
-    rewrite xorb_true_r.
-    reflexivity.
+  apply Int64.same_bits_eq.
+  intros i Hi.
+  repeat rewrite Int64.bits_xor ; try assumption.
+  repeat rewrite Int64.bits_or ; try assumption.
+  unfold Int64.mone.
+  repeat rewrite Int64.testbit_repr ; try assumption.
+  repeat rewrite Z.shiftl_spec ; try lia.
+  destruct i as [ | i' | i' ] ; try reflexivity.
+  repeat rewrite Z.lnot_spec ; try lia.
+  rewrite xorb_true_r.
+  reflexivity.
 Qed.
